src/lib/communication/DY.Lib.Communication.API.Lemmas.fst
@@ -1,0 +1,155 @@
+module DY.Lib.Communication.API.Lemmas
+
+open Comparse
+open DY.Core
+open DY.Lib.Crypto.PkEncryption.Split
+open DY.Lib.State.PKI
+open DY.Lib.State.PrivateKeys
+
+open DY.Lib.Communication.API
+open DY.Lib.Communication.API.Predicates
+
+#set-options "--fuel 0 --ifuel 0 --z3cliopt 'smt.qi.eager_threshold=100'"
+
+val encrypt_message_proof:
+  {|cinvs:crypto_invariants|} ->
+  tr:trace ->
+  sender:principal -> receiver:principal -> payload:bytes ->
+  pk:bytes -> nonce:bytes ->
+  Lemma
+  (requires
+    has_communication_layer_invariants cinvs /\
+    is_knowable_by (join (principal_label sender) (principal_label receiver)) tr payload /\
+    is_secret (principal_label sender) tr nonce /\
+    PkNonce? (get_usage nonce) /\
+    is_encryption_key (PkKey comm_layer_tag empty) (principal_label receiver) tr pk
+  )
+  (ensures
+    is_publishable tr (encrypt_message sender receiver payload pk nonce)
+  )
+let encrypt_message_proof #cinvs tr sender receiver payload pk nonce =
+  let msg = {sender; receiver; payload} in
+  let msg_encrypted = encrypt_message sender receiver payload pk nonce in
+  
+  serialize_wf_lemma communication_message (is_knowable_by (join (principal_label sender) (principal_label receiver)) tr) msg;
+  serialize_wf_lemma communication_message (bytes_invariant tr) msg;
+  assert(bytes_invariant tr (serialize communication_message msg));
+  
+  assert(match get_sk_usage pk with
+    | PkKey pkenc_tag _ ->
+        pkenc_tag = comm_layer_tag ==>
+          pkenc_pred.pred tr pk (serialize communication_message msg) == 
+            (pkenc_crypto_predicates_communication_layer cinvs.usages).pred tr pk (serialize communication_message msg)
+    | _ -> True);
+
+  assert(cinvs.preds.pkenc_pred.pred tr pk (serialize communication_message msg));
+  assert(bytes_invariant tr msg_encrypted);
+  ()
+
+val send_confidential_proof:
+  {|invs:protocol_invariants|} ->
+  tr:trace -> 
+  keys_sess_ids:communication_keys_sess_ids ->
+  sender:principal -> receiver:principal -> payload:bytes ->
+  Lemma
+  (requires
+    trace_invariant tr /\ has_pki_invariant invs /\ has_communication_layer_invariants invs.crypto_invs /\
+    is_knowable_by (join (principal_label sender) (principal_label receiver)) tr payload
+  )
+  (ensures (
+    let (_, tr_out) = send_confidential keys_sess_ids sender receiver payload tr in
+    trace_invariant tr_out
+  ))
+let send_confidential_proof #invs tr keys_sess_ids sender receiver payload =
+  match get_public_key sender keys_sess_ids.pki (PkEnc comm_layer_tag) receiver tr with
+  | (None, tr) -> ()
+  | (Some pk_receiver, tr) -> (
+    let (nonce, tr) = mk_rand PkNonce (principal_label sender) 32 tr in
+    encrypt_message_proof tr sender receiver payload pk_receiver nonce;
+    ()
+  )
+
+
+val decrypt_message_proof:
+  {|cinvs:crypto_invariants|} ->
+  tr:trace ->
+  receiver:principal -> sk_receiver:bytes -> msg_encrypted:bytes ->  
+  Lemma
+  (requires
+    has_communication_layer_invariants cinvs /\
+    is_decryption_key (PkKey comm_layer_tag empty) (principal_label receiver) tr sk_receiver /\
+    bytes_invariant tr msg_encrypted
+  )
+  (ensures (
+    match decrypt_message sk_receiver msg_encrypted with
+    | None -> True
+    | Some {sender; receiver=receiver'; payload} -> (
+      let Some msg_plain = pk_dec sk_receiver msg_encrypted in
+      (//
+        // /\
+        //get_sk_label (Pk sk_receiver) == principal_label receiver /\
+        is_knowable_by (join (principal_label sender) (principal_label receiver)) tr payload ///\
+        //(pkenc_pred.pred tr (Pk sk_receiver) msg_plain \/
+        //is_publishable tr msg_plain)
+        //is_corrupt tr (principal_label receiver)
+      )
+    )
+  ))
+let decrypt_message_proof #cinvs tr receiver sk_receiver msg_encrypted =
+  match decrypt_message sk_receiver msg_encrypted with
+  | None -> ()
+  | Some {sender; receiver=receiver'; payload} -> ( 
+    let Some msg_plain = pk_dec sk_receiver msg_encrypted in
+    let pk = pk sk_receiver in
+    
+    assert(get_usage sk_receiver == PkKey comm_layer_tag empty);
+ 
+    // This follows from the precondition:
+    // has_communication_layer_invariants invs.crypto_invs
+    assert(match get_sk_usage pk with
+          | PkKey pkenc_tag _ ->
+            pkenc_tag = comm_layer_tag ==>
+              pkenc_pred.pred tr pk msg_plain == 
+                (pkenc_crypto_predicates_communication_layer cinvs.usages).pred tr pk msg_plain
+          | _ -> True
+    );
+    // Since the precondition states that pk has the
+    // comm_layer_tag, we can directly assert that the
+    // predicates are equal.
+    assert(pkenc_pred.pred tr pk msg_plain == 
+                (pkenc_crypto_predicates_communication_layer cinvs.usages).pred tr pk msg_plain);
+
+    // From the crypto predicates we can infer that the
+    // payload can flow to the sender and the receiver
+    assert((pkenc_crypto_predicates_communication_layer cinvs.usages).pred tr pk msg_plain ==>
+          (match parse communication_message msg_plain with
+            | Some {sender; receiver; payload} -> (
+              get_sk_label pk == principal_label receiver /\
+              (get_label payload) `can_flow tr` (join (principal_label sender) (principal_label receiver))
+            )
+            | None -> False)
+    );
+
+    FStar.Classical.move_requires (parse_wf_lemma communication_message (is_publishable tr)) msg_plain;
+    FStar.Classical.move_requires (parse_wf_lemma communication_message (bytes_invariant tr)) msg_plain;
+    assert(bytes_invariant tr payload);
+    assert(is_knowable_by (join (principal_label sender) (principal_label receiver)) tr payload \/
+      is_publishable tr payload);
+
+    assert(is_knowable_by (join (principal_label sender) (principal_label receiver)) tr payload);
+    ()
+  )
+
+val receive_confidential_proof:
+  {|invs:protocol_invariants|} -> tr:trace -> comm_keys_ids:communication_keys_sess_ids ->
+  receiver:principal -> msg_id:timestamp ->
+  Lemma
+  (requires
+    trace_invariant tr /\ 
+    has_private_keys_invariant invs
+  )
+  (ensures (
+    let (_, tr_out) = receive_confidential comm_keys_ids receiver msg_id tr in
+    trace_invariant tr_out
+  ))
+let receive_confidential_proof #invs tr comm_keys_ids receiver msg_id = ()
