src/lib/communication/DY.Lib.Communication.API.fst
@@ -1,0 +1,117 @@
+module DY.Lib.Communication.API
+
+open Comparse
+open DY.Core
+open DY.Lib.State.PKI
+open DY.Lib.State.PrivateKeys
+open DY.Lib.Event.Typed
+
+#set-options "--fuel 0 --ifuel 0 --z3cliopt 'smt.qi.eager_threshold=100'"
+
+(*** Messages ***)
+
+[@@with_bytes bytes]
+type communication_message = {
+  sender:principal;
+  receiver:principal;  
+  payload:bytes;
+}
+
+%splice [ps_communication_message] (gen_parser (`communication_message))
+%splice [ps_communication_message_is_well_formed] (gen_is_well_formed_lemma (`communication_message))
+
+instance parseable_serializeable_bytes_communication_message: parseable_serializeable bytes communication_message
+  = mk_parseable_serializeable ps_communication_message
+
+(*** Events ***)
+
+#push-options "--ifuel 1 --fuel 0"
+[@@with_bytes bytes]
+type communication_event =
+  | CommunicationLayerSendMsg: sender:principal -> receiver:principal -> payload:bytes -> communication_event
+  | CommunicationLayerReceiveMsg: sender:principal -> receiver:principal -> payload:bytes -> communication_event
+
+%splice [ps_communication_event] (gen_parser (`communication_event))
+%splice [ps_communication_event_is_well_formed] (gen_is_well_formed_lemma (`communication_event))
+
+
+instance event_communication_event: event communication_event = {
+  tag = "DY.Lib.Communication.Event";
+  format = mk_parseable_serializeable ps_communication_event;
+}
+
+(*** Layer Setup ***)
+
+val comm_layer_tag: string
+let comm_layer_tag = "DY.Lib.Communication.PublicKey"
+
+(*** Communication Layer ***)
+
+(**** Layer Initialization ****)
+
+type communication_keys_sess_ids = {
+  pki: state_id;
+  private_keys: state_id;
+}
+
+val initialize_communication: principal -> principal -> traceful (option (communication_keys_sess_ids & communication_keys_sess_ids))
+let initialize_communication sender receiver =
+  let* client_global_session_priv_key_id = initialize_private_keys sender in
+  generate_private_key sender client_global_session_priv_key_id (PkDec "DY.Lib.Communication.PublicKey");*
+
+  let* receiver_global_session_priv_key_id = initialize_private_keys receiver in
+  generate_private_key receiver receiver_global_session_priv_key_id (PkDec "DY.Lib.Communication.PublicKey");*
+
+  let*? priv_key_receiver = get_private_key receiver receiver_global_session_priv_key_id (PkDec "DY.Lib.Communication.PublicKey") in
+  let pub_key_receiver = pk priv_key_receiver in
+  let* client_global_session_pub_key_id = initialize_pki sender in
+  install_public_key sender client_global_session_pub_key_id (PkEnc "DY.Lib.Communication.PublicKey") receiver pub_key_receiver;*
+
+  let*? priv_key_client = get_private_key sender client_global_session_priv_key_id (PkDec "DY.Lib.Communication.PublicKey") in
+  let pub_key_client = pk priv_key_client in
+  let* receiver_global_session_pub_key_id = initialize_pki receiver in
+  install_public_key receiver receiver_global_session_pub_key_id (PkEnc "DY.Lib.Communication.PublicKey") sender pub_key_client;*
+
+  let client_comm_keys_sess_ids = {pki=client_global_session_pub_key_id; private_keys=client_global_session_priv_key_id} in
+  let receiver_comm_keys_sess_ids = {pki=receiver_global_session_pub_key_id; private_keys=receiver_global_session_priv_key_id} in
+  return (Some (client_comm_keys_sess_ids, receiver_comm_keys_sess_ids))
+
+
+(**** Confidential Send and Receive Functions ****)
+
+val encrypt_message: principal -> principal -> bytes -> bytes -> bytes -> bytes
+let encrypt_message sender receiver payload pk nonce =
+  let msg = {sender; receiver; payload} in
+  let msg_bytes = serialize communication_message msg in
+  pk_enc pk nonce msg_bytes
+
+val send_confidential: 
+  communication_keys_sess_ids ->
+  principal -> principal -> bytes ->
+  traceful (option timestamp)
+let send_confidential keys_sess_ids sender receiver payload =
+  let*? pk_receiver = get_public_key sender keys_sess_ids.pki (PkEnc "DY.Lib.Communication.PublicKey") receiver in
+  let* nonce = mk_rand PkNonce (principal_label sender) 32 in
+  let msg_encrypted = encrypt_message sender receiver payload pk_receiver nonce in
+  let* msg_id = send_msg msg_encrypted in  
+  return (Some msg_id)
+
+
+val decrypt_message: bytes -> bytes -> option communication_message
+let decrypt_message sk_receiver msg_encrypted =
+  let? msg_plain_bytes = pk_dec sk_receiver msg_encrypted in
+  let? msg_plain = parse communication_message msg_plain_bytes in
+  Some msg_plain
+
+val receive_confidential:
+  communication_keys_sess_ids ->
+  principal -> timestamp ->
+  traceful (option communication_message)
+let receive_confidential keys_sess_ids receiver msg_id =
+  let*? sk_receiver = get_private_key receiver keys_sess_ids.private_keys (PkDec "DY.Lib.Communication.PublicKey") in
+  let*? msg_encrypted = recv_msg msg_id in
+  let*? msg_plain:communication_message = return (decrypt_message sk_receiver msg_encrypted) in
+  return (Some msg_plain)
+
+
+(**** Confidential and Authenticated Send and Receive Functions ****)
